src/Examples/Interval/Example_Interval_DG_Flagship.thy
@@ -333,7 +333,8 @@ definition flagship_graph_config ::
       show_internal_globals = False,
       owner_of = (\<lambda>_. ''main''),
       cluster_label = (\<lambda>_ _. ''main / root context''),
-      source_text = Some (pretty_string_of_program Map.empty [] (prog_main flagship_prog))
+      source_text = Some (pretty_string_of_program Map.empty [] (prog_main flagship_prog)),
+      node_annotation = (\<lambda>_. None)
     \<rparr>"
 
 definition flagship_graph_domain :: "(pp \<times> unit + unit) list" where
