src/Examples/Interval/Example_Interval_DG_IP_Flagship.thy
@@ -340,7 +340,8 @@ definition twice_graph_config ::
       show_internal_globals = False,
       owner_of = compiled_owner_of twice_pi twice_procs ''main'' twice_main,
       cluster_label = (\<lambda>owner _. owner @ '' / context=unit''),
-      source_text = Some (pretty_string_of_program twice_pi twice_procs twice_main)
+      source_text = Some (pretty_string_of_program twice_pi twice_procs twice_main),
+      node_annotation = (\<lambda>_. None)
     \<rparr>"
 
 definition twice_graph_domain :: "(pp \<times> unit + unit) list" where
