src/Examples/Tooling/Example_Mixed_Sign_Interval_GraphViz.thy
@@ -83,7 +83,8 @@ definition mixed_graphviz_graph_config ::
       show_internal_globals = False,
       owner_of = (\<lambda>_. ''main''),
       cluster_label = (\<lambda>_ _. ''mixed Sign answers''),
-      source_text = Some (pretty_string_of_program (\<lambda>_. None) [] (prog_main mixed_graphviz_prog))
+      source_text = Some (pretty_string_of_program (\<lambda>_. None) [] (prog_main mixed_graphviz_prog)),
+      node_annotation = (\<lambda>_. None)
     \<rparr>"
 
 definition mixed_graphviz_graph_domain :: "(pp \<times> unit + unit) list" where
